Simplify defn. of RC semantics

linking/rc_semantics.v
@@ -49,49 +49,27 @@ Variable sem : @EffectSem (Genv.t F V) C.
 
 Record state : Type := 
   mk { core :> C
-     ; args : list val
-     ; rets : list val
      ; locs : block -> bool }.
 
 Definition updC (c : C) (st : state) :=
   match st with
-    | mk _ args rets locs => mk c args rets locs 
+    | mk _ locs => mk c locs 
   end.
 
 Definition upd_locs locs (st : state) :=
   match st with
-    | mk c args rets _ => mk c args rets locs 
+    | mk c _ => mk c locs 
   end.
 
 Definition initial_core ge v vs := 
   match initial_core sem ge v vs with
-    | Some c => Some (mk c vs nil (fun _ => false))
+    | Some c => Some (mk c (getBlocks vs))
     | None => None
   end.
 
-Lemma initial_core_args ge v vs c : 
-  initial_core ge v vs = Some c -> 
-  args c = vs.
-Proof.
-unfold initial_core.
-case_eq (core_semantics.initial_core sem ge v vs).
-solve[intros c0 H; inversion 1; subst; simpl; auto].
-solve[intros _; inversion 1].
-Qed.
-
-Lemma initial_core_rets ge v vs c : 
-  initial_core ge v vs = Some c -> 
-  rets c = nil.
-Proof.
-unfold initial_core.
-case_eq (core_semantics.initial_core sem ge v vs).
-solve[intros c0 H; inversion 1; subst; simpl; auto].
-solve[intros _; inversion 1].
-Qed.
-
 Lemma initial_core_locs ge v vs c : 
   initial_core ge v vs = Some c -> 
-  locs c = (fun _ : block => false).
+  locs c = getBlocks vs.
 Proof.
 unfold initial_core.
 case_eq (core_semantics.initial_core sem ge v vs).
@@ -112,8 +90,8 @@ Definition after_external ov c :=
   match after_external sem ov (core c) with
     | Some c' => 
       match ov with 
-        | Some v => Some (mk c' (args c) (v :: rets c) (locs c))
-        | None => Some (mk c' (args c) (rets c) (locs c))
+        | Some v => Some (mk c' (fun b => getBlocks (v::nil) b || locs c b))
+        | None => Some (mk c' (locs c))
       end
     | None => None
   end.
@@ -127,10 +105,7 @@ Definition halted c :=
 Arguments halted /.
 
 Definition roots F V (ge : Genv.t F V) (c : state) := 
-  fun b => isGlobalBlock ge b
-        || getBlocks (args c) b
-        || getBlocks (rets c) b
-        || locs c b.
+  fun b => isGlobalBlock ge b || locs c b.
 
 Lemma roots_domains_eq 
     F1 F2 V1 V2 (ge1 : Genv.t F1 V1) (ge2 : Genv.t F2 V2) c b : 
@@ -150,11 +125,8 @@ Definition reach_set (ge : Genv.t F V) (c : state) (m : mem) :=
 Definition effstep ge U c m c' m' :=
   effstep sem ge U (core c) m (core c') m' 
   /\ (forall b ofs, U b ofs=true -> reach_set ge c m b=true)
-  /\ args c'=args c
-  /\ rets c'=rets c
-  /\ locs c' = fun b => StructuredInjections.freshloc m m' b
-                     || reach_set ge c m b
-                     || reach_set ge c m' b.
+  /\ locs c' = REACH m' (fun b => StructuredInjections.freshloc m m' b
+                               || reach_set ge c m b).
 
 Arguments effstep /.
 
@@ -182,25 +154,10 @@ Proof.
 unfold after_external; case (core_semantics.after_external _ _).
 intros ?; inversion 1; subst; unfold roots; simpl.
 extensionality b.
-rewrite <-(orb_comm (getBlocks (v :: rets c) b)).
+rewrite (orb_assoc (getBlocks (v :: nil) b)).
 symmetry.
-rewrite <-(orb_assoc (isGlobalBlock ge b)).
-rewrite (orb_comm (isGlobalBlock ge b)).
-rewrite (orb_comm (getBlocks (args c) b)).
-rewrite <-(orb_assoc (getBlocks (rets c) b)).
-rewrite <-(orb_assoc (getBlocks (rets c) b)).
-rewrite <-orb_assoc.
-rewrite orb_assoc.
-change
-   ((fun b => getBlocks (v :: nil) b || getBlocks (rets c) b) b
-   || (getBlocks (args c) b || (isGlobalBlock ge b || locs c b)) =
-   getBlocks (v :: rets c) b || (isGlobalBlock ge b || getBlocks (args c) b)
-   || locs c b).
-rewrite <-getBlocks_app; simpl.
-rewrite <-orb_assoc.
-symmetry.
-rewrite (orb_comm (isGlobalBlock ge b)).
-rewrite <-orb_assoc; auto.
+rewrite (orb_comm (getBlocks (v :: nil) b)).
+rewrite (orb_assoc (isGlobalBlock ge b)); auto.
 inversion 1.
 Qed.
   
@@ -243,7 +200,7 @@ Lemma my_effax1 M ge c m c' m' :
   corestep ge c m c' m'  
   /\ Mem.unchanged_on (fun b ofs => M b ofs = false) m m'.
 Proof.
-destruct 1 as [H [H2 [H3 [H4 H5]]]]; split.
+destruct 1 as [H [H2 H3]]; split.
 exists M; split; auto.
 apply effax1 in H. destruct H; auto.
 Qed.
@@ -257,7 +214,7 @@ Lemma my_effstep_valid M ge c m c' m' :
   effstep ge M c m c' m' ->
   forall b z, M b z = true -> Mem.valid_block m b.
 Proof.
-destruct 1 as [H [H2 [H3 [H4 H5]]]].
+destruct 1 as [H [H2 H3]].
 intros b ofs. eapply effstep_valid; eauto.
 Qed.
 
